src/NewTypeVariable.v
@@ -28,6 +28,9 @@ Require Import LibTactics.
 Inductive new_tv_ty : ty -> id -> Prop :=
 | new_tv_con : forall i i' : id, new_tv_ty (con i') i
 | new_tv_var : forall i i' : id, i < i' -> new_tv_ty (var i) i'
+| new_tv_appl : forall (tau tau' : ty) (i : id), new_tv_ty tau i ->
+                                             new_tv_ty tau' i ->
+                                             new_tv_ty (appl tau tau') i
 | new_tv_arrow : forall (tau tau' : ty) (i : id), new_tv_ty tau i ->
                                              new_tv_ty tau' i ->
                                              new_tv_ty (arrow tau tau') i.
@@ -49,9 +52,11 @@ Lemma new_tv_ty_ids : forall (st : id) (tau : ty),
     forall x : id, in_list_id x (ids_ty tau) = true -> x < st.
 Proof.
   induction tau; intros; simpl in *; mysimp; intuition.
-  destruct (eq_id_dec i x); intuition. inversion H. omega.
-  apply in_list_id_or_append_inversion in H0.
-  destruct H0; inversion H; auto.
+  - destruct (eq_id_dec i x); intuition. inversion H. omega.
+  - apply in_list_id_or_append_inversion in H0.
+    destruct H0; inversion H; auto.
+  - apply in_list_id_or_append_inversion in H0.
+    destruct H0; inversion H; auto.
 Qed.
 
 Hint Resolve new_tv_ty_ids.
@@ -61,14 +66,14 @@ Lemma add_subst_new_tv_ty : forall (s : substitution) (st : id) (tau1 tau2 : ty)
 Proof.
   induction s; crush. 
   rewrite apply_subst_nil.
-  induction tau1; crush.
-  inverts* H; intuition. 
-  inverts* H.
-  fequals; eauto.
   induction tau1; crush;
-  inverts* H; intuition. 
-  inverts* H.
-  fequals; eauto.
+    try inverts* H; intuition; 
+    try inverts* H;
+    fequals; eauto.
+    induction tau1; crush;
+      inverts* H; intuition; 
+    inverts* H;
+    fequals; eauto.
 Qed.
 
 Hint Resolve add_subst_new_tv_ty.
@@ -77,10 +82,10 @@ Hint Rewrite add_subst_new_tv_ty:RE.
 Lemma new_tv_ty_trans_le : forall (tau : ty) (st1 st2 : id),
     new_tv_ty tau st1 -> st1 <= st2 -> new_tv_ty tau st2.
 Proof.
-  induction tau; crush.
-  inverts* H.
-  econstructor. omega.
-  inverts* H.
+  induction tau; crush;
+  try inverts* H.
+  try econstructor; omega;
+  try inverts* H.
 Qed.
 
 Hint Resolve new_tv_ty_trans_le.
@@ -91,6 +96,10 @@ Lemma new_tv_compose_subst_type : forall (s s1 s2 : substitution) (st : id) (tau
   induction tau.
   - crush.
   - crush.
+  - intros.
+    simpl.
+    inverts* H0.
+    fequals; eauto.
   - intros.
     simpl.
     inverts* H0.
@@ -106,6 +115,9 @@ Inductive new_tv_schm : schm -> id -> Prop :=
 | new_tv_sc_con : forall i i' : id, new_tv_schm (sc_con i') i
 | new_tv_sc_var : forall i i' : id, i < i' -> new_tv_schm (sc_var i) i'
 | new_tv_sc_gen : forall i i' : id, new_tv_schm (sc_gen i') i
+| new_tv_sc_appl : forall (tau tau' : schm) (i : id), new_tv_schm tau i ->
+                                               new_tv_schm tau' i ->
+                                               new_tv_schm (sc_appl tau tau') i
 | new_tv_sc_arrow : forall (tau tau' : schm) (i : id), new_tv_schm tau i ->
                                                new_tv_schm tau' i ->
                                                new_tv_schm (sc_arrow tau tau') i.
@@ -118,13 +130,9 @@ Hint Constructors new_tv_schm.
 Lemma new_tv_ty_to_schm : forall tau st,
     new_tv_schm (ty_to_schm tau) st <-> new_tv_ty tau st.
 Proof.
-  intros. split.
-  induction tau; simpl in *; try inversion H; try econstructor; eauto.
-  inverts* H.
-  inverts* H.
-  inverts* H.
-  intros.
-  induction tau; simpl in *; try inversion H; try econstructor; eauto.
+  intros. split;
+  induction tau; simpl in *; try inversion H; try econstructor; eauto;
+  try inverts* H.
 Qed.
 
 Hint Resolve new_tv_ty_to_schm.
@@ -158,15 +166,22 @@ Proof.
     econstructor; eauto. 
     inversion H0.
     inversion H0.
+  - inversion H.
+    subst.
+    cases (apply_inst_subst (compute_inst_subst x i) sigma1).
+    cases (apply_inst_subst (compute_inst_subst x i) sigma2).
+    inversion H0.
+    econstructor; eauto. 
+    inversion H0.
+    inversion H0.
 Qed.
 
 Hint Resolve new_tv_schm_to_new_tv_ty.
 
 Lemma new_tv_schm_plus : forall sigma st st', new_tv_schm sigma st -> new_tv_schm sigma (st + st').
 Proof.
-  induction sigma; intros; try econstructor; eauto.
-  inversion H. subst. auto.
-  inversion H. subst. eauto.
+  induction sigma; intros; try econstructor; eauto;
+  inversion H; subst; auto.
   Unshelve. apply x.
 Qed.
 
@@ -184,10 +199,10 @@ Hint Resolve new_tv_schm_Succ.
 Lemma new_tv_schm_trans : forall st st' sigma,
     new_tv_schm sigma st -> st <= st' -> new_tv_schm sigma st'.
 Proof.
-  induction sigma; crush.
-  inversion H.
-  econstructor; crush. 
-  inverts* H.
+  induction sigma; crush;
+  try inversion H;
+  try econstructor; crush; 
+  try inverts* H.
 Qed.
 
 Hint Resolve new_tv_schm_trans.
@@ -199,10 +214,12 @@ Proof.
   intros.
   induction sigma;
   mysimp.
-  cases (find_subst s i0); eauto;
+  - cases (find_subst s i0); eauto;
   try inversion H; omega.
-  inversion H. subst.
-  fequals; eauto.
+  - inversion H. subst.
+    fequals; eauto.
+  - inversion H. subst.
+    fequals; eauto.
 Qed.
   
 Hint Resolve new_tv_schm_apply_subst.
@@ -234,6 +251,22 @@ Proof.
      rewrite Nat.add_comm.
      eapply find_subst_id_compute; eauto.
      inversion H2.
+   - intros. 
+     inversion H. subst.
+     simpl in H0. rewrite apply_subst_schm_appl in H2.
+     edestruct (exist_appl_apply_inst_appl (compute_inst_subst st p)); eauto.
+     destruct H3.
+     edestruct (exist_appl_apply_inst_appl x); eauto.
+     destruct H4. subst.
+     apply and_appl_apply_inst_appl in H1.
+     destruct H1.
+     apply and_appl_apply_inst_appl in H2.
+     destruct H2.
+     simpl.
+     eapply Nat.max_lub_r in H0 as H0r.
+     eapply Nat.max_lub_l in H0 as H0l.
+     erewrite <- IHsigma1; eauto.
+     erewrite <- IHsigma2; eauto.
    - intros. 
      inversion H. subst.
      simpl in H0. rewrite apply_subst_schm_arrow in H2.
@@ -298,6 +331,17 @@ Proof.
     reflexivity.
   - crush.
   - crush.
+  - inverts* H6.
+    simpl.
+    fequals; eauto.
+    fequals; eauto.
+    fequals; eauto.
+    apply IHsigma1 in H2.
+    repeat rewrite <- apply_subst_ctx_eq in H2.
+    inversion H2; eauto.
+    apply IHsigma2 in H4.
+    repeat rewrite <- apply_subst_ctx_eq in H4.
+    inversion H4; eauto.
   - inverts* H6.
     simpl.
     fequals; eauto.
@@ -394,13 +438,18 @@ Lemma new_tv_gen_aux_ty: forall (tau : ty) (G : ctx) (st : id) l,
     new_tv_ty tau st -> new_tv_ctx G st -> new_tv_schm (fst (gen_ty_aux tau G l)) st.
 Proof.
   induction tau; crush.
-  cases (in_list_id i (FV_ctx G)); crush.
-  cases (index_list_id i l); crush.
-  inverts* H.
-  eapply IHtau1 with (G:= G) (l:=l) in H3; eauto.
-  cases (gen_ty_aux tau1 G l); crush.
-  eapply IHtau2 with (G:= G) (l:=l0) in H5; eauto.
-  cases (gen_ty_aux tau2 G l0); crush.
+  - cases (in_list_id i (FV_ctx G)); crush.
+    cases (index_list_id i l); crush.
+  - inverts* H.
+    eapply IHtau1 with (G:= G) (l:=l) in H3; eauto.
+    cases (gen_ty_aux tau1 G l); crush.
+    eapply IHtau2 with (G:= G) (l:=l0) in H5; eauto.
+    cases (gen_ty_aux tau2 G l0); crush.
+  - inverts* H.
+    eapply IHtau1 with (G:= G) (l:=l) in H3; eauto.
+    cases (gen_ty_aux tau1 G l); crush.
+    eapply IHtau2 with (G:= G) (l:=l0) in H5; eauto.
+    cases (gen_ty_aux tau2 G l0); crush.
 Qed.
 
 Hint Resolve new_tv_gen_aux_ty.
@@ -434,54 +483,79 @@ Lemma new_ty_to_cons_new_tv_subst : forall tau i a s,
     a < i -> new_tv_ty tau i -> new_tv_subst s i -> new_tv_subst ((a, tau) :: s) i.
 Proof.
   induction tau; intros; simpl in *. 
-  inversion H0. subst.
-  inversion H1.
-  econstructor. intros.
-  subst.
-  simpl in H6. 
-  destruct (eq_id_dec a x). subst.
-  assumption.
-  simpl in H6. 
-  apply in_list_id_append_comm_true in H6.
-  unfold img_ids in H6. simpl in H6. destruct (eq_id_dec i x).
-  subst. assumption. fold (img_ids s) in H6.
-  apply in_list_id_append_comm_true in H6.
-  fold (FV_subst s) in H6. auto.
-  econstructor. intros.
-  simpl in H2.
-  destruct (eq_id_dec a x). subst.
-  assumption.
-  apply in_list_id_append_comm_true in H2.
-  unfold img_ids in H2. simpl in H2. 
-  fold (img_ids s) in H2.
-  apply in_list_id_append_comm_true in H2.
-  fold (FV_subst s) in H2. 
-  inversion H1. auto.
-  inversion H0. subst.
-  econstructor. intros.
-  crush.
-  apply in_list_id_append_comm_true in H2.
-  unfold img_ids in H2. simpl in H2. 
-  fold (img_ids s) in H2.
-  assert (new_tv_subst ((a, tau1) :: s) i). auto.
-  assert (new_tv_subst ((a, tau2) :: s) i). auto.
-  inversion H3. subst.
-  inversion H5. subst.
-  specialize H7 with (x:=x).
-  specialize H8 with (x:=x).
-  simpl in *. destruct (eq_id_dec a x); eauto.
-  unfold img_ids in *. simpl in *.
-  fold (img_ids s) in *.
-  apply in_list_id_append_comm_true in H2.
-  rewrite <- app_assoc in H2.
-  rewrite app_assoc in H2.
-  apply in_list_id_append_comm_true2 in H2.
-  rewrite app_assoc in H2.
-  apply in_list_id_or_append_inversion in H2.
-  destruct H2.
-  rewrite <- app_assoc in H2.
-  auto.
-  auto.
+  - inversion H0. subst.
+    inversion H1.
+    econstructor. intros.
+    subst.
+    simpl in H6. 
+    destruct (eq_id_dec a x). subst.
+    assumption.
+    simpl in H6. 
+    apply in_list_id_append_comm_true in H6.
+    unfold img_ids in H6. simpl in H6. destruct (eq_id_dec i x).
+    subst. assumption. fold (img_ids s) in H6.
+    apply in_list_id_append_comm_true in H6.
+    fold (FV_subst s) in H6. auto.
+  - econstructor. intros.
+    simpl in H2.
+    destruct (eq_id_dec a x). subst.
+    assumption.
+    apply in_list_id_append_comm_true in H2.
+    unfold img_ids in H2. simpl in H2. 
+    fold (img_ids s) in H2.
+    apply in_list_id_append_comm_true in H2.
+    fold (FV_subst s) in H2. 
+    inversion H1. auto.
+  - inversion H0. subst.
+    econstructor. intros.
+    crush.
+    apply in_list_id_append_comm_true in H2.
+    unfold img_ids in H2. simpl in H2. 
+    fold (img_ids s) in H2.
+    assert (new_tv_subst ((a, tau1) :: s) i). auto.
+    assert (new_tv_subst ((a, tau2) :: s) i). auto.
+    inversion H3. subst.
+    inversion H5. subst.
+    specialize H7 with (x:=x).
+    specialize H8 with (x:=x).
+    simpl in *. destruct (eq_id_dec a x); eauto.
+    unfold img_ids in *. simpl in *.
+    fold (img_ids s) in *.
+    apply in_list_id_append_comm_true in H2.
+    rewrite <- app_assoc in H2.
+    rewrite app_assoc in H2.
+    apply in_list_id_append_comm_true2 in H2.
+    rewrite app_assoc in H2.
+    apply in_list_id_or_append_inversion in H2.
+    destruct H2.
+    rewrite <- app_assoc in H2.
+    auto.
+    auto.
+  - inversion H0. subst.
+    econstructor. intros.
+    crush.
+    apply in_list_id_append_comm_true in H2.
+    unfold img_ids in H2. simpl in H2. 
+    fold (img_ids s) in H2.
+    assert (new_tv_subst ((a, tau1) :: s) i). auto.
+    assert (new_tv_subst ((a, tau2) :: s) i). auto.
+    inversion H3. subst.
+    inversion H5. subst.
+    specialize H7 with (x:=x).
+    specialize H8 with (x:=x).
+    simpl in *. destruct (eq_id_dec a x); eauto.
+    unfold img_ids in *. simpl in *.
+    fold (img_ids s) in *.
+    apply in_list_id_append_comm_true in H2.
+    rewrite <- app_assoc in H2.
+    rewrite app_assoc in H2.
+    apply in_list_id_append_comm_true2 in H2.
+    rewrite app_assoc in H2.
+    apply in_list_id_or_append_inversion in H2.
+    destruct H2.
+    rewrite <- app_assoc in H2.
+    auto.
+    auto.
 Qed.
 
 Hint Resolve new_ty_to_cons_new_tv_subst.
@@ -496,17 +570,17 @@ Proof.
   unfold img_ids in *.
   specialize H1 with (x:=x).
   induction tau.
-  simpl in *. destruct (eq_id_dec a x). eauto.
+  - simpl in *. destruct (eq_id_dec a x). eauto.
   rewrite arrowcons.
   rewrite <- app_assoc.
   apply in_list_id_append_comm_true3.
   simpl. destruct (eq_id_dec i0 x); eauto.
-  crush.
-  crush.
+  - crush.
+  - crush.
+  - crush.
 Qed.
 
 Hint Resolve new_tv_subst_tail.
-
 Lemma new_tv_subst_arrow_inversion : forall a tau1 tau2 s i,
     new_tv_subst ((a, arrow tau1 tau2) :: s) i ->
     new_tv_subst ((a, tau1)::s) i /\ new_tv_subst ((a, tau2)::s) i.
@@ -546,21 +620,64 @@ Proof.
 Qed.
 
 Hint Resolve new_tv_subst_arrow_inversion.
+
+Lemma new_tv_subst_appl_inversion : forall a tau1 tau2 s i,
+    new_tv_subst ((a, appl tau1 tau2) :: s) i ->
+    new_tv_subst ((a, tau1)::s) i /\ new_tv_subst ((a, tau2)::s) i.
+Proof.
+  intros.
+  inverts* H.
+  split.
+  - econstructor.
+    intros. apply H0. 
+    unfold FV_subst in *.
+    unfold img_ids in *.
+    simpl (concat (map ids_ty (img ((a, appl tau1 tau2) :: s)))).
+    simpl (dom ((a, appl tau1 tau2) :: s)).
+    simpl (dom ((a, tau1) :: s)) in H.
+    simpl (concat (map ids_ty (img ((a, tau1) :: s)))) in H.
+    rewrite <- app_assoc.
+    apply in_list_id_append_comm_true3 in H.
+    apply in_list_id_append_comm_true3.
+    apply in_list_id_or_append_inversion in H.
+    destruct H.
+    apply in_list_id_append1; eauto.
+    apply in_list_id_append2; eauto.
+  - econstructor.
+    intros. apply H0. 
+    unfold FV_subst in *.
+    unfold img_ids in *.
+    simpl (concat (map ids_ty (img ((a, appl tau1 tau2) :: s)))).
+    simpl (dom ((a, appl tau1 tau2) :: s)).
+    simpl (dom ((a, tau2) :: s)) in H.
+    simpl (concat (map ids_ty (img ((a, tau2) :: s)))) in H.
+    apply in_list_id_append_comm_true3 in H.
+    apply in_list_id_append_comm_true3.
+    apply in_list_id_or_append_inversion in H.
+    destruct H.
+    apply in_list_id_append1; eauto.
+    apply in_list_id_append2; eauto.
+Qed.
+
+Hint Resolve new_tv_subst_appl_inversion.
     
 Lemma new_tv_subst_cons_new_tv_ty : forall tau s i a,
     new_tv_subst ((a, tau) :: s) i -> new_tv_ty tau i.
 Proof.
   induction tau; crush.
-  econstructor.
-  inversion H. subst.
-  apply H0. 
-  unfold FV_subst.
-  unfold img_ids.
-  eapply in_list_id_append_comm_true.
-  crush.
-  apply new_tv_subst_arrow_inversion in H as H'.
-  destruct H'.
-  eauto.
+  - econstructor.
+    inversion H. subst.
+    apply H0. 
+    unfold FV_subst.
+    unfold img_ids.
+    eapply in_list_id_append_comm_true.
+    crush.
+  - apply new_tv_subst_appl_inversion in H as H'.
+    destruct H'.
+    eauto.
+  - apply new_tv_subst_arrow_inversion in H as H'.
+    destruct H'.
+    eauto.
 Qed.
 
 Hint Resolve new_tv_subst_cons_new_tv_ty.
@@ -577,12 +694,15 @@ Lemma new_tv_apply_subst_ty : forall (st : id) (s : substitution) (tau : ty),
     new_tv_ty tau st -> new_tv_subst s st -> new_tv_ty (apply_subst s tau) st.
 Proof.
   induction tau; intros.
-  inversion H; subst. eauto.
-  inverts* H.
-  crush.
-  inverts* H.
-  simpl.
-  econstructor; eauto.
+  - inversion H; subst. eauto.
+  - inverts* H.
+    crush.
+  - inverts* H.
+    simpl.
+    econstructor; eauto.
+  - inverts* H.
+    simpl.
+    econstructor; eauto.
 Qed.
 
 Hint Resolve new_tv_apply_subst_ty.
@@ -606,13 +726,16 @@ Lemma new_tv_apply_subst_schm : forall (st : id) (s : substitution) (sigma : sch
     new_tv_schm sigma st -> new_tv_subst s st -> new_tv_schm (apply_subst_schm s sigma) st.
 Proof.
   induction sigma; intros.
-  inverts* H.
-  crush.
-  simpl.
-  auto.
-  inverts* H.
-  simpl.
-  econstructor; eauto.
+  - inverts* H.
+  - crush.
+  - simpl.
+    auto.
+  - inverts* H.
+    simpl.
+    econstructor; eauto.
+  - inverts* H.
+    simpl.
+    econstructor; eauto.
 Qed.
 
 Hint Resolve new_tv_apply_subst_schm.
